Proved the uniqueness

Semigroup.v
@@ -8,7 +8,6 @@ Section Test.
   Infix "+!" := Aplus (at level 50, left associativity).
   Variable Aplus_assoc : forall x y z : A, (x +! y) +! z = x +! (y +! z).
   Variable Aplus_comm : forall x y, x +! y = y +! x.
-  Variable Aeq_dec : forall x y : A, {x = y} + {x <> y}.
 
   Inductive ExpA :=
   | ExpVar : nat -> ExpA
@@ -37,6 +36,7 @@ Section Test.
         end
       | _ => constr:(S n, (x, n)::table)
       end
+    | Some ?n' => constr:(n, table)
     end.
 
   Ltac gen_table x y :=
@@ -66,16 +66,11 @@ Section Test.
 
   Fixpoint ins n (nf : NFA) : NFA :=
     match nf with
-    | nil =>
-      match n with
-      | O => 1 :: nil
-      | S n' => (repeat O (S n')) ++ (1 :: nil)
-      end
+    | nil => n :: nil
     | m::nf' =>
-      match n with
-      | O => (S m) :: nf'
-      | S n' => m :: ins n' nf'
-      end
+      if le_dec n m
+        then n :: m :: nf'
+        else m :: ins n nf'
     end.
 
   Fixpoint exp2nf' (ex : ExpA)(nf : NFA) : NFA :=
@@ -100,25 +95,155 @@ Section Test.
     | ExpPlus ey ez => exp2A ey table +! exp2A ez table
     end.
 
-  Lemma repeat_inj : forall X (x : X) n m, repeat x n = repeat x m -> n = m.
+  Fixpoint nf2A nf table :=
+    match nf with
+    | nil => bot
+    | n::nil => getKey n table
+    | n::nf' => getKey n table +! nf2A nf' table
+    end.
+
+  Fixpoint addnf a nf table :=
+    match nf with
+    | nil => a
+    | n::nf' => getKey n table +! addnf a nf' table
+    end.
+
+  Lemma addnf_plus : forall table a b nf,
+    addnf (a +! b) nf table = a +! addnf b nf table.
   Proof with simpl in *.
-    induction n; destruct m; (discriminate || firstorder).
-    f_equal... inversion H. firstorder.
+    induction nf; [auto|]...
+    rewrite IHnf. repeat rewrite <- Aplus_assoc. rewrite (Aplus_comm a). auto.
   Qed.
 
-  Lemma ins_inj : forall n m nf, ins n nf = ins m nf -> n = m.
+  Lemma addnf_comm : forall table a b nf,
+    a +! addnf b nf table = b +! addnf a nf table.
   Proof with simpl in *.
-    induction n; intros...
-    - destruct nf; destruct m; (discriminate || auto)...
-      inversion H. exfalso. omega.
-    - destruct nf; destruct m; simpl in *; (discriminate || auto)...
-      inversion H. f_equal. apply app_inv_tail in H1. eauto using repeat_inj.
-      inversion H. exfalso. omega.
-      inversion H. firstorder.
+    intros. rewrite <- addnf_plus. rewrite Aplus_comm. rewrite addnf_plus. auto.
   Qed.
 
-  Axiom uniq : forall ex ey table , exp2nf ex = exp2nf ey -> exp2A ex table = exp2A ey table.
-  (* TODO: proof *)
+  Lemma addnf_nf2A : forall table n nf,
+    addnf (getKey n table) nf table = nf2A (n::nf) table.
+  Proof with simpl in *.
+    induction nf; [auto|]... rewrite IHnf.
+    destruct nf.
+    - auto.
+    - repeat rewrite <- Aplus_assoc. f_equal. auto.
+  Qed.
+
+  Lemma addnf_left : forall table a n nf,
+    addnf a (n::nf) table = a +! nf2A (n::nf) table.
+  Proof with simpl in*.
+    intros.
+    rewrite <- (addnf_nf2A table n nf).
+    induction nf; simpl in *; [auto|].
+    rewrite (Aplus_comm (getKey a0 table)).
+    repeat rewrite <- Aplus_assoc. rewrite IHnf.
+    repeat rewrite Aplus_assoc. f_equal. auto.
+  Qed.
+
+  Lemma nf2A_ins : forall table n nf,
+    nf2A (ins n nf) table = nf2A (n::nf) table.
+  Proof with simpl in *.
+    induction n; induction nf...
+    - auto.
+    - auto.
+    - auto.
+    - destruct (le_dec (S n) a)...
+      + auto.
+      + f_equal. rewrite IHnf.
+        destruct nf...
+        * auto.
+        * destruct (le_dec (S n) n1); simpl; repeat rewrite <- Aplus_assoc; f_equal; auto.
+  Qed.
+
+  Require Import Recdef.
+
+  Function list_ind2' X (P : list X -> Prop) (H : P nil) (H0 : forall x, P (x :: nil))
+    (H1 : forall x y l, P (y :: l) -> P (x :: y :: l)) l {measure length l} : P l :=
+    match l return P l with
+    | nil => H
+    | x::nil => H0 x
+    | x::y::l' => H1 x y l' (list_ind2' P H H0 H1 (y :: l'))
+    end.
+  Proof.
+    intros. subst. auto.
+  Qed.
+
+  Definition list_ind2 : forall X (P : list X -> Prop),
+    P nil ->
+    (forall x, P (x :: nil)) ->
+    (forall x y l, P (y:: l) -> (P (x :: y :: l))) ->
+    forall l, P l := fun X P H H0 H1 l => list_ind2' P H H0 H1 l.
+
+  Lemma exp2nf'_cons : forall ex nf,
+    exp2nf' ex nf <> nil.
+  Proof with simpl in *.
+    induction ex; induction nf...
+    - discriminate.
+    - destruct (le_dec n a); discriminate.
+    - intro. firstorder.
+    - intro. firstorder.
+  Qed.
+
+  Lemma nf_inj : forall ex nf table,
+    addnf (exp2A ex table) nf table = nf2A (exp2nf' ex nf) table.
+  Proof with simpl in *.
+    induction ex.
+    - apply (list_ind2 (fun nf => forall table,
+    addnf (exp2A (ExpVar n) table) nf table = nf2A (exp2nf' (ExpVar n) nf) table)); intros...
+      + auto.
+      + destruct (le_dec n x); simpl; auto.
+      + specialize (H table).
+        destruct (le_dec n x); destruct (le_dec n y)...
+        * repeat rewrite <- Aplus_assoc. rewrite (Aplus_comm (getKey n table)).
+          repeat rewrite Aplus_assoc. f_equal. auto.
+        * rewrite H. rewrite nf2A_ins...
+          destruct l...
+          { rewrite (Aplus_comm (getKey y table)). repeat rewrite <- Aplus_assoc.
+            f_equal. auto. }
+          { destruct (le_dec n n1); repeat rewrite <- Aplus_assoc; f_equal;
+            rewrite (Aplus_comm (getKey n table)); repeat rewrite Aplus_assoc; f_equal; auto. }
+        * f_equal. auto.
+        * rewrite H. auto.
+    - apply (list_ind2 (fun nf => forall (table : list (A * nat)),
+addnf (exp2A (ExpPlus ex1 ex2) table) nf table =
+nf2A (exp2nf' (ExpPlus ex1 ex2) nf) table)); intros...
+      + rewrite <- IHex2.
+        destruct (exp2nf' ex1 nil) eqn:?.
+        { apply exp2nf'_cons in Heqn. contradiction. }
+        rewrite addnf_left. rewrite Aplus_comm. f_equal.
+        rewrite <- Heqn. rewrite <- IHex1... auto.
+      + rewrite <- IHex2.
+        destruct (exp2nf' ex1 (x :: nil)) eqn:?.
+        { apply exp2nf'_cons in Heqn. contradiction. }
+        rewrite addnf_left. rewrite <- Heqn. rewrite <- IHex1...
+        rewrite (Aplus_comm (exp2A ex1 table)). repeat rewrite <- Aplus_assoc.
+        f_equal. auto.
+      + rewrite H. rewrite <- (IHex2 (exp2nf' ex1 (x :: y :: l))).
+        destruct (exp2nf' ex1 (x :: y :: l)) eqn:?.
+        { apply exp2nf'_cons in Heqn. contradiction. }
+        rewrite addnf_left. rewrite <- Heqn. rewrite <- IHex1.
+        rewrite addnf_left. simpl. rewrite <- Aplus_assoc. rewrite <- Aplus_assoc.
+        rewrite (Aplus_comm _ (getKey x table)). rewrite Aplus_assoc. f_equal.
+        rewrite <- IHex2.
+        destruct (exp2nf' ex1 (y :: l)) eqn:?.
+        { apply exp2nf'_cons in Heqn1. contradiction. }
+        rewrite addnf_left. rewrite <- Heqn1. rewrite Aplus_assoc. f_equal.
+        rewrite <- IHex1. rewrite addnf_left. auto.
+  Qed.
+
+  Lemma uniq' : forall table ex ey nf,
+    exp2nf' ex nf = exp2nf' ey nf ->
+    addnf (exp2A ex table) nf table = addnf (exp2A ey table) nf table.
+  Proof with simpl in *.
+    intros. rewrite nf_inj. rewrite nf_inj. rewrite H. auto.
+  Qed.
+
+  Lemma uniq : forall ex ey table,
+    exp2nf ex = exp2nf ey -> exp2A ex table = exp2A ey table.
+  Proof with simpl in *.
+    unfold exp2nf. intros. apply (uniq' table) in H... auto.
+  Qed.
 
   Ltac semigroup :=
     match goal with
@@ -142,6 +267,19 @@ Section Test.
   Qed.
 
   Goal forall x y z w, (x +! y) +! (z +! w) = w +! (x +! z) +! y.
+  Proof.
+    intros.
+    semigroup.
+  Qed.
+
+  Goal forall x y z, x +! y +! x +! z = x +! x +! y +! z.
+  Proof.
+    intros.
+    semigroup.
+  Qed.
+
+  Goal forall x y z w,
+    (x +! y) +! (x +! z +! (w +! y) +! w) = w +! w +! z +! y +! y+! x +! x.
   Proof.
     intros.
     semigroup.
